GreedyDeriv/Examples.lean
@@ -19,93 +19,112 @@ instance : Coe String (Loc Char) where
 def r : Regex (Char) := plus 'a' "ab"
 #eval r.matchEnd "ab"
 #eval r.gmatch "ab"
+#eval r.greedy "ab"
 
 -- (a + ab)*
 def r2 : Regex (Char) := (plus 'a' "ab").star false
 #eval r2.matchEnd "aab"
 #eval r2.gmatch "aab"
+#eval r2.greedy "aab"
 
 -- c + ab
 def r3 : Regex (Char) := plus 'c' (mul 'a' 'b')
 #eval r3.matchEnd "ab"
 #eval r3.gmatch "ab"
+#eval r3.greedy "ab"
 
 -- (a + aa)a
 def r4 : Regex (Char) := (plus 'a' "aa").mul 'a'
 #eval r4.matchEnd "aaa"
 #eval r4.gmatch "aaa"
+#eval r4.greedy "aaa"
 
 -- a*a
 def r5 : Regex (Char) := (star 'a' false).mul 'a'
 #eval r5.matchEnd "aa"
 #eval r5.gmatch "aa"
+#eval r5.greedy "aa"
 
 -- (ε + b)*
 def r6 : Regex (Char) := (epsilon.plus 'b').star false
 #eval r6.matchEnd "bb"
 #eval r6.gmatch "bb"
+#eval r6.greedy "bb"
 
 -- (ε + b)(ε + b)*
 def r6' : Regex (Char) := (epsilon.plus 'b').mul ((epsilon.plus 'b').star false)
 #eval r6'.matchEnd "bb"
 #eval r6'.gmatch "bb"
+#eval r6'.greedy "bb"
 
 -- (a + ε + b)*
 def r7 : Regex (Char) := (plus 'a' (epsilon.plus 'b')).star false
 #eval r7.matchEnd "aaaabbb"
 #eval r7.gmatch "aaaabbb"
+#eval r7.greedy "aaaabbb"
 
 -- (ε + a)b
 def r8 : Regex (Char) := (epsilon.plus 'a').mul 'b'
 #eval r8.matchEnd "ab"
 #eval r8.gmatch "ab"
+#eval r8.greedy "ab"
 
 -- ((a + ε + b) + b)
 def r9 : Regex (Char) := Regex.plus ((plus 'a' epsilon).plus 'b') 'b'
 #eval r9.gmatch "b"
+#eval r9.greedy "b"
 #eval r9.matchEnd "b"
 
 -- (ε + a)*b
 def r10 : Regex (Char) := ((Regex.plus epsilon 'a').star false).mul 'b'
 #eval r10.gmatch "ab"
+#eval r10.greedy "ab"
 #eval r10.matchEnd "ab"
 
 -- (a + ε)*(ε + b)
 def r11 : Regex (Char) := ((Regex.plus 'a' epsilon).star false).mul (Regex.plus (epsilon) 'b')
 #eval r11.gmatch "ab"
+#eval r11.greedy "ab"
 #eval r11.matchEnd "ab"
 
 -- (ε + a)*(ε + b)
 def r12 : Regex (Char) := ((Regex.plus epsilon 'a').star false).mul (Regex.plus (epsilon) 'b')
 #eval r12.gmatch "ab"
+#eval r12.greedy "ab"
 #eval r12.matchEnd "ab"
 
 -- (a + ε + b)*b
 def r13 : Regex (Char) := ((Regex.plus 'a' (Regex.plus epsilon 'b')).star false).mul 'b'
 #eval r13.gmatch "bb"
+#eval r13.greedy "bb"
 #eval r13.matchEnd "bb"
 
 -- a*?a
 def r14 : Regex (Char) := (star 'a' true).mul 'a'
 #eval r14.matchEnd "aaa"
 #eval r14.gmatch "aaa"
+#eval r14.greedy "aaa"
 
 -- a*?b
 def r15 : Regex (Char) := (star 'a' true).mul 'b'
 #eval r15.matchEnd "aab"
 #eval r15.gmatch "aab"
+#eval r15.greedy "aab"
 
 -- (a + ε + b)*?b
 def r16 : Regex (Char) := (star (plus 'a' (plus epsilon 'b')) true).mul 'b'
 #eval r16.matchEnd "aabb"
 #eval r16.gmatch "aabb"
+#eval r16.greedy "aabb"
 
 -- (aa + aaa)*
 def r17 : Regex (Char) := (star (plus "aa" "aaa") false)
 #eval r17.matchEnd "aaa"
 #eval r17.gmatch "aaa"
+#eval r17.greedy "aaa"
 
 -- (a + b*?)*
 def r18 : Regex Char := (star (plus 'a' (star 'b' true)) false)
 #eval r18.matchEnd "aaabbb"
 #eval r18.gmatch "aaabbb"
+#eval r18.greedy "aaabbb"
